Axiomatising host_apply_impl_m by refactoring

WebAssembly/Wasm_Interpreter_Monad_Config.thy
@@ -1,62 +1,53 @@
-theory Wasm_Monad_Assertions 
-  imports Wasm_Interpreter_Monad "../libs/Misc_Generic_Lemmas" "../libs/List_Assn" begin
-(* separation logic methods *)
+theory Wasm_Interpreter_Monad_Config imports  Wasm_Countable Wasm_Interpreter 
+  "HOL-Imperative_HOL.Array" 
+  "../libs/Byte_Array"   "../libs/List_Assn" begin 
 
-method extract_list_idx for i :: nat =
-  (subst listI_assn_extract[of i], (simp;fail), (simp;fail))
-  
-method reinsert_list_idx for i :: nat =
-  rule listI_assn_reinsert[where i=i] listI_assn_reinsert'[where i=i],
-  (frame_inference; fail),
-  (simp;fail),
-  (simp;fail)
+instance uint8 :: heap ..
+instance tf :: heap ..
+instance v :: heap ..
+instance global_ext :: (heap) heap ..
 
-method extract_reinsert_list_idx for i :: nat uses heap = 
- extract_pre_pure?, extract_list_idx i, sep_auto heap:heap, extract_pre_pure?, reinsert_list_idx i
+type_synonym mem_m = "(byte_array) \<times> nat option"
 
-lemma list_assn_basic_heap_rule: 
-  assumes "<P_i> c <Q>"
-    "P_i = P (xs!i) (ys!i) * F" "\<And>r. Q r \<Longrightarrow>\<^sub>A  P_i * R r" "i < length xs"
-  shows "<list_assn P xs ys * F> c <\<lambda>r. list_assn P xs ys * F * R r>"
-  unfolding list_assn_conv_idx
-  apply(insert assms(2, 4))
-  apply(extract_list_idx i)
-  apply(sep_auto heap:assms(1))
-  apply(rule ent_trans[OF fr_refl[OF assms(3)]])
-  apply(reinsert_list_idx i)
-  apply(sep_auto)
-  done
+record inst_m = \<comment> \<open>instances\<close>
+  types :: "tf array"
+  funcs :: "i array"
+  tabs :: "i array"
+  mems :: "i array"
+  globs :: "i array"
 
-lemmas is_complex_goal = asm_rl[of "< _ > _ < _ >"] asm_rl[of "_ \<Longrightarrow>\<^sub>A _"]
+instance inst_m_ext :: (countable) countable
+proof(rule countable_classI[of "\<lambda>i. to_nat (inst_m.types i, inst_m.funcs i, inst_m.tabs i, inst_m.mems i, inst_m.globs i, inst_m.more i)"])
+qed auto
 
-method_setup then_else = \<open>let
-in
-  Method.text_closure -- Method.text_closure -- Method.text_closure >>
-    (fn ((textb, textt), texte) => fn ctxt => fn using => fn st =>
-      let
-        val bmethod = Method.evaluate_runtime textb ctxt using;
-        val tmethod = Method.evaluate_runtime textt ctxt using;
-        val emethod = Method.evaluate_runtime texte ctxt using;
-      in
-        (case try (fn st => bmethod st |> Seq.pull) st of
-          SOME (SOME (Seq.Result st,_)) => tmethod st
-        | _ => emethod st)
-      end)
-end     
-\<close>
+datatype cl_m = \<comment> \<open>function closures\<close>
+  Func_native inst_m (cl_m_type:tf) "t list" "b_e list"
+| Func_host (cl_m_type:tf) host
 
-method defer_vcg = then_else \<open>rule is_complex_goal\<close> \<open>fail\<close> 
-  \<open>find_goal \<open>rule is_complex_goal\<close>, 
-  (rule is_complex_goal | tactic \<open>defer_tac 1\<close>)\<close>
+instance cl_m :: countable
+  by (countable_datatype)
 
-method sep_auto_all = (defer_vcg | (rule is_complex_goal, sep_auto))+
+instance cl_m :: heap ..
 
+type_synonym tabinst_m = "(i option) array \<times> nat option"
 
+record s_m = \<comment> \<open>store\<close>
+  funcs :: "cl_m array"
+  tabs :: "tabinst_m array"
+  mems :: "mem_m array"
+  globs :: "global array"
 
-abbreviation "expect_assn A B x_opt y_opt \<equiv> (case x_opt of 
-  Some x \<Rightarrow> (case y_opt of Some y \<Rightarrow> A x y | None \<Rightarrow> false)
-  | None \<Rightarrow> (case y_opt of Some y \<Rightarrow> false | None \<Rightarrow> B)
-  )"
+instance s_m_ext :: (countable) countable
+proof(rule countable_classI[of "\<lambda>i. to_nat (s_m.funcs i, s_m.tabs i, s_m.mems i, s_m.globs i, s_m.more i)"])
+qed auto
+
+instance s_m_ext :: (heap) heap ..
+
+(* 0: redex, 1: label contexts, 2: frame arity, 3: frame *)
+datatype frame_context_m = Frame_context_m redex "label_context list" (frame_arity:nat) (f_locs_m:"v array") (f_inst_m:"inst_m")
+
+datatype config_m = Config_m depth s_m frame_context_m "frame_context_m list"
+
 
 
 (* assertions *) 
@@ -143,50 +134,10 @@ definition cfg_m_assn :: "inst_assocs \<Rightarrow> config \<Rightarrow> config_
 
 
 
-lemma cl_m_agree_type: "cl_m_agree i_s cl cl_m \<Longrightarrow> cl_type cl = cl_m_type cl_m"
-  unfolding cl_m_agree_def cl_m_agree_j_def cl_type_def cl_m_type_def
-  by (auto, simp split:cl.splits cl_m.splits)
+abbreviation "expect_assn A B x_opt y_opt \<equiv> (case x_opt of 
+  Some x \<Rightarrow> (case y_opt of Some y \<Rightarrow> A x y | None \<Rightarrow> false)
+  | None \<Rightarrow> (case y_opt of Some y \<Rightarrow> false | None \<Rightarrow> B)
+  )"
 
-
-lemma [sep_heap_rules]: "<tabinst_m_assn t t_m> 
-    Array.len (fst t_m) 
-    <\<lambda>r. tabinst_m_assn t t_m * \<up>(r=length (fst t))>"
-  unfolding tabinst_m_assn_def
-  by (sep_auto split: prod.splits)
-
-lemma [sep_heap_rules]: "<tabinst_m_assn t t_m> 
-    Array.nth (fst t_m) x
-    <\<lambda>r. tabinst_m_assn t t_m * \<up>(r=(fst t)!x)>"
-  unfolding tabinst_m_assn_def
-  by (sep_auto split: prod.splits)
-
-lemma [sep_heap_rules]: "<mem_m_assn m mi> 
-    len_byte_array (fst mi) 
-    <\<lambda>r. mem_m_assn m mi * \<up>(r=mem_length m)>"
-  unfolding mem_m_assn_def mem_length_def mem_rep_length_def
-  by (sep_auto split: prod.splits)
-
-(* misc triples *)
-
-abbreviation "fits_at_in l n la \<equiv> (length l > 0 \<longrightarrow> n+length l \<le> length la)"
-
-abbreviation "insert_at_in l n la \<equiv> take n la @ l @ drop (n+length l) la"
-
-lemma list_blit_array_triple:
-  "<a \<mapsto>\<^sub>a la> 
-  list_blit_array l a n
-  <\<lambda>r. \<up>(fits_at_in l n la) 
-    * a \<mapsto>\<^sub>a insert_at_in l n la>"
-proof(induct l arbitrary:a la n)
-case Nil
-  then show ?case by sep_auto
-next
-  case (Cons a l)
-  show ?case 
-    supply [simp del] = list_blit_array.simps
-    apply(subst list_blit_array.simps)
-    apply(sep_auto heap:Cons split:list.splits simp: take_update_last)
-    done
-qed
 
 end
